src/coq/Utils/ListUtil.v
@@ -1451,10 +1451,133 @@ Proof.
       right. assumption.
 Qed.
 
+
+Lemma Forall2_map_impl {A B C} : forall (P:A -> C -> Prop) (Q:B -> C -> Prop) (f:A -> B),
+    (forall a c, P a c -> Q (f a) c) ->
+    forall (l1 : list A) (l2 : list C) , Forall2 P l1 l2 -> Forall2 Q (map f l1) l2.
+Proof.
+  intros ? ? ? Himpl ? ? Hforall.
+  induction Hforall; cbn; constructor; eauto.
+Qed.
+
+  Lemma Forall2_map_r {A B C} : forall (P: A -> B -> Prop) (f:C -> B),
+      forall (l1 : list A) (l2 : list C) , Forall2 P l1 (map f l2) <-> Forall2 (fun x y => P x (f y)) l1 l2.
+  Proof.
+    intros P f l1 l2.
+    split; intros H.
+    - remember (map f l2) as l3.
+      revert l2 Heql3.
+      induction H; intros l2 EQ.
+      + symmetry in EQ.
+        apply map_eq_nil in EQ. subst.
+        constructor.
+      + symmetry in EQ.
+        apply map_eq_cons in EQ.
+        destruct EQ as [c [tl [EQ1 [EQ2 M]]]].
+        subst.
+        constructor; auto.
+    - induction H; simpl; auto.
+  Qed.
+
+  Lemma Forall2_map_l {A B C} : forall (P: A -> B -> Prop) (f:C -> A),
+      forall (l1 : list C) (l2 : list B) , Forall2 P (map f l1) l2 <-> Forall2 (fun x y => P (f x) y) l1 l2.
+  Proof.
+    intros P f l1 l2.
+    split; intros H.
+    - remember (map f l1) as l3.
+      revert l1 Heql3.
+      induction H; intros l1 EQ.
+      + symmetry in EQ.
+        apply map_eq_nil in EQ. subst.
+        constructor.
+      + symmetry in EQ.
+        apply map_eq_cons in EQ.
+        destruct EQ as [c [tl [EQ1 [EQ2 M]]]].
+        subst.
+        constructor; auto.
+    - induction H; simpl; auto.
+  Qed.
+
+  Lemma Forall2_eq {A} : 
+      forall (l1 : list A) (l2 : list A) , Forall2 eq l1 l2 <-> l1 = l2.
+  Proof.
+    intros l1 l2.
+    split; intros H.
+    - induction H; subst; auto.
+    - revert l2 H.
+      induction l1; intros l2 EQ; subst; auto.
+  Qed.
+
+  Lemma Forall2_ext_m : forall {A B} (f : A -> OOM B)
+      xs ys1 ys2,
+        Forall2 (fun a b => f a = NoOom b) xs ys1 ->
+        Forall2 (fun a b => f a = NoOom b) xs ys2 ->
+        ys1 = ys2.
+  Proof.
+    intros A B f xs ys1 ys2 H H0. 
+    revert ys2 H0.
+    induction H; intros ys2 F; inversion F; subst; auto.
+    rewrite H in H3. inversion H3; subst.
+    rewrite (IHForall2 l'0 H5).
+    reflexivity.
+  Qed.
+
+Lemma Forall2_inj_l :
+  forall A B (f : A -> B) (g : A -> B) (l1 l2 : list A) (l : list B)
+    (HINJ : forall a, In a l1 -> forall a', f a = g a' -> a' = a )
+    (HL1: Forall2 (fun a b => f a = b) l1 l)
+    (HL2: Forall2 (fun a b => g a = b) l2 l),
+    l1 = l2.
+Proof.
+  intros A B f g l1 l2 l HINJ HL1.
+  revert l2.
+  induction HL1; intros l2 HL2; inversion HL2; subst; auto.
+  assert (In x (x::l)) by (left; auto).
+  eapply (HINJ x) with (a':=x0) in H; auto; subst.
+  forward IHHL1.
+  - intros; subst. eapply HINJ; eauto. right.  assumption.
+  - rewrite (IHHL1 l0 H4).
+    reflexivity.
+Qed.
+
+  Lemma Forall2_inj_OOM_l :
+    forall A B (f : A -> OOM B) (g : A -> OOM B) (l1 l2 : list A) (l : list B)
+      (HINJ : forall a, In a l1 -> forall a' b, f a = NoOom b -> g a' = NoOom b -> a' = a )
+      (HL1: Forall2 (fun a b => f a = NoOom b) l1 l)
+      (HL2: Forall2 (fun a b => g a = NoOom b) l2 l),
+      l1 = l2.
+  Proof.
+    intros A B f g l1 l2 l HINJ HEQ1 HEQ2.
+    rewrite <- (Forall2_map_r (fun a b => f a = b) NoOom) in HEQ1.
+    rewrite <- (Forall2_map_r (fun a b => g a = b) NoOom) in HEQ2.
+    eapply Forall2_inj_l; eauto.
+    intros.
+    rewrite (Forall2_map_r (fun a b => f a = b) NoOom) in HEQ1.
+    destruct (Forall2_In _ a _ _ H HEQ1) as [b [_ HB]].
+    eapply HINJ; eauto.
+    rewrite <- H0.
+    auto.
+  Qed.
+
+
+  Lemma Forall2_repeat_OOM : forall {A B} (f : A -> OOM B) (a:A) (b:B) n (l:list B),
+      f a = ret b ->
+      Forall2 (fun a b => f a = ret b) (repeat a n) l ->
+      l = repeat b n.
+  Proof.
+    intros A B f a b n l EQ F. 
+    revert l EQ F.
+    induction n; intros; cbn in *.
+    - inversion F. reflexivity.
+    - inversion F; subst.
+      rewrite EQ in H1. inversion H1; subst.
+      rewrite (IHn l'); auto.
+  Qed.
+
+
 (* Better behaved version of Forall that can be used in recursive functions *)
 Definition FORALL {A} (P : A -> Prop) (l : list A) :=
   List.fold_right (fun x b => P x /\ b) True l.
-
 
 Lemma FORALL_forall : forall {A} (P : A -> Prop) (l:list A),
     FORALL P l <-> Forall P l.
@@ -1481,3 +1604,108 @@ Proof.
     + right. intros C. apply n. intuition.
 Qed.
 
+
+Inductive Forall2T {A B : Type} (f : A -> B -> Type) : list A -> list B -> Type :=
+| Forall2T_nil : Forall2T f [] []
+| Forall2T_cons : forall a b l1 l2, (f a b) * Forall2T f l1 l2 -> Forall2T f (a::l1) (b::l2).
+
+  Lemma map_monad_oom_Forall2T : forall {A B : Type} (f : A -> OOM B) (l : list A) (res : list B),
+      map_monad f l = NoOom res -> Forall2T (fun (a : A) (b : B) => f a = NoOom b) l res.
+  Proof.
+    induction l; intros.
+    - cbn in H. inversion H; subst. constructor.
+    - cbn in H.
+      repeat break_match_hyp_inv.
+      constructor. split; auto.
+  Qed.
+
+  Lemma Forall2T_InT_r :
+    forall {A B} (f : A -> B -> Type) (l1 : list A) (l2 : list B),
+      Forall2T f l1 l2 -> forall b,
+        InT b l2 -> { a : A & f a b * InT a l1}%type.
+  Proof.
+    intros A B.
+    fix IH 4.
+    intros f l1 l2 H; inversion H; subst; clear H; intros x HX.
+    - inversion HX.
+    - inversion HX; subst.
+      + destruct X as [HF HL].
+        exists a. split; auto. left. auto.
+      + destruct X as [_ HL].
+        destruct (IH _ _ _ HL x X0) as [c [HFC HR]].
+        exists c. split; auto. right. assumption.
+  Qed.
+
+  
+  (*
+  Lemma Forall2T_map_r1 {A B C} : forall (P: A -> B -> Prop) (f:C -> B),
+      forall (l1 : list A) (l2 : list C) , Forall2T (fun x y => P x (f y)) l1 l2 -> Forall2T P l1 (map f l2).
+  Proof.
+    intros P f l1 l2 H.
+    induction H; simpl; auto.
+    constructor.
+    constructor. 
+
+  
+  Lemma Forall2T_map_r {A B C} : forall (P: A -> B -> Prop) (f:C -> B),
+      forall (l1 : list A) (l2 : list C) , Forall2T P l1 (map f l2) -> Forall2T (fun x y => P x (f y)) l1 l2.
+  Proof.
+    intros P f l1 l2.
+    split; intros H.
+    - remember (map f l2) as l3.
+      revert l2 Heql3.
+      induction H; intros l2 EQ.
+      + symmetry in EQ.
+        apply map_eq_nil in EQ. subst.
+        constructor.
+      + symmetry in EQ.
+        apply map_eq_cons in EQ.
+        destruct EQ as [c [tl [EQ1 [EQ2 M]]]].
+        subst.
+        constructor; auto.
+    - induction H; simpl; auto.
+  Qed.
+
+  Lemma Forall2_map_l {A B C} : forall (P: A -> B -> Prop) (f:C -> A),
+      forall (l1 : list C) (l2 : list B) , Forall2 P (map f l1) l2 <-> Forall2 (fun x y => P (f x) y) l1 l2.
+  Proof.
+    intros P f l1 l2.
+    split; intros H.
+    - remember (map f l1) as l3.
+      revert l1 Heql3.
+      induction H; intros l1 EQ.
+      + symmetry in EQ.
+        apply map_eq_nil in EQ. subst.
+        constructor.
+      + symmetry in EQ.
+        apply map_eq_cons in EQ.
+        destruct EQ as [c [tl [EQ1 [EQ2 M]]]].
+        subst.
+        constructor; auto.
+    - induction H; simpl; auto.
+  Qed.
+
+  Lemma Forall2_eq {A} : 
+      forall (l1 : list A) (l2 : list A) , Forall2 eq l1 l2 <-> l1 = l2.
+  Proof.
+    intros l1 l2.
+    split; intros H.
+    - induction H; subst; auto.
+    - revert l2 H.
+      induction l1; intros l2 EQ; subst; auto.
+  Qed.
+
+  Lemma Forall2_ext_m : forall {A B} (f : A -> OOM B)
+      xs ys1 ys2,
+        Forall2 (fun a b => f a = NoOom b) xs ys1 ->
+        Forall2 (fun a b => f a = NoOom b) xs ys2 ->
+        ys1 = ys2.
+  Proof.
+    intros A B f xs ys1 ys2 H H0. 
+    revert ys2 H0.
+    induction H; intros ys2 F; inversion F; subst; auto.
+    rewrite H in H3. inversion H3; subst.
+    rewrite (IHForall2 l'0 H5).
+    reflexivity.
+  Qed.
+*)
